src/tls/MITLS.Repr.ClientHello.fst
@@ -27,24 +27,81 @@ module MITLS.Repr.ClientHello
 module LP = LowParse.Low.Base
 module B = LowStar.Monotonic.Buffer
 module HS = FStar.HyperStack
-module R = MITLS.Repr
+module R = LowParse.Repr
 module CH = Parsers.ClientHello
+module C = LowStar.ConstBuffer
+module R_CHE = MITLS.Repr.ClientHelloExtensions
 open FStar.Integers
 open FStar.HyperStack.ST
 
-let t = CH.clientHello
+let ptr = R.repr_ptr_p CH.clientHello CH.clientHello_parser
+let pos (b:R.const_slice) = R.repr_pos_p CH.clientHello b CH.clientHello_parser
 
-let repr (b:R.const_slice) =
-  R.repr_p CH.clientHello b CH.clientHello_parser32
-
-let version (#b:R.const_slice) (r:repr b)
+/// Reader for the protocol version
+///   returns a value, since this is a leaf reader
+let version (p:ptr)
   : Stack Parsers.ProtocolVersion.protocolVersion
-    (requires R.valid r)
+    (requires R.valid p)
     (ensures fun h0 pv h1 ->
       B.modifies B.loc_none h0 h1 /\
-      pv == CH.((R.value r).version))
-  = let open R in
-    R.reveal_valid();
-    let b = R.to_slice b in
-    let pos = CH.accessor_clientHello_version b r.start_pos in
+      pv == (R.value p).CH.version)
+  = R.reveal_valid();
+    let b = R.temp_slice_of_repr_ptr p in
+    let pos = CH.accessor_clientHello_version b 0ul in
     Parsers.ProtocolVersion.protocolVersion_reader b pos
+
+/// To read a field from a positional repr,
+/// just use the pointer reader
+let pos_version (#b:R.const_slice) (r:pos b)
+  : Stack Parsers.ProtocolVersion.protocolVersion
+    (requires R.repr_pos_valid r)
+    (ensures fun h0 pv h1 ->
+      B.modifies B.loc_none h0 h1 /\
+      pv == (R.value_pos r).CH.version)
+  = version (R.as_ptr r)
+
+/// Accessor for the extensions
+///    returns a pointer, since it is a variable-length field
+///    and offsets to enable positional representations
+inline_for_extraction
+private
+let extensions' (p:ptr)
+  : Stack (R_CHE.ptr & uint_32 & uint_32)
+    (requires R.valid p)
+    (ensures fun h0 (e_ptr, pos, len) h1 ->
+      B.modifies B.loc_none h0 h1 /\
+      R.valid e_ptr h1 /\
+      R.value e_ptr == (R.value p).CH.extensions /\
+      (R.Ptr?.b e_ptr `C.const_sub_buffer pos len` (R.Ptr?.b p)))
+  = R.reveal_valid();
+    let b = R.temp_slice_of_repr_ptr p in
+    let pos = CH.accessor_clientHello_extensions b 0ul in
+    let pos_to = Parsers.ClientHelloExtensions.clientHelloExtensions_jumper b pos in
+    let e_ptr = R.mk b pos pos_to Parsers.ClientHelloExtensions.clientHelloExtensions_parser32 in
+    e_ptr,
+    pos,
+    pos_to - pos
+
+/// Accessor for the extensions
+///    returns a pointer, since it is a variable-length field
+let extensions (p:ptr)
+  : Stack R_CHE.ptr
+    (requires R.valid p)
+    (ensures fun h0 e_ptr h1 ->
+      B.modifies B.loc_none h0 h1 /\
+      R.valid e_ptr h1 /\
+      R.value e_ptr == (R.value p).CH.extensions /\
+      e_ptr `R.sub_ptr` p)
+  =  let e_ptr, _, _ = extensions' p in e_ptr
+
+/// Just for demo purposes: to access a field from a positional repr,
+/// just use the pointer accessor
+let pos_extensions (#b:R.const_slice) (r:pos b)
+  : Stack (R_CHE.pos b)
+    (requires R.repr_pos_valid r)
+    (ensures fun h0 es h1 ->
+      B.modifies B.loc_none h0 h1 /\
+      R.repr_pos_valid es h1)
+  = let p, pos, len = extensions' (R.as_ptr r) in
+    let open R in
+    R.as_repr_pos b (r.start_pos + pos) (r.start_pos + pos + len) p
