src/tls/MITLS.Repr.Handshake.fst
@@ -21,13 +21,13 @@ module MITLS.Repr.Handshake
    This module encapsulates wire-format representations of
    Parsers.Handshake messages.
 
-   Its main type, `repr b` is an instance of MITLS.Repr.repr
+   Its main type, `ptr` is an instance of MITLS.Repr.repr_ptr
    instantiated with serverHello_parser
 *)
 module LP = LowParse.Low.Base
 module B = LowStar.Monotonic.Buffer
 module HS = FStar.HyperStack
-module R = MITLS.Repr
+module R = LowParse.Repr
 module HSM = Parsers.Handshake
 module RCH = MITLS.Repr.ClientHello
 module RSH = MITLS.Repr.ServerHello
@@ -36,88 +36,91 @@ open FStar.HyperStack.ST
 
 let t = HSM.handshake
 
-let repr (b:R.const_slice) =
-  R.repr_p t b HSM.handshake_parser32
+let ptr = R.repr_ptr_p t HSM.handshake_parser
 
-let handshakeType (#b:R.const_slice) (r:repr b)
+let pos (b:R.const_slice) = R.repr_pos_p t b HSM.handshake_parser
+
+let handshakeType (p:ptr)
   : Stack Parsers.HandshakeType.handshakeType
     (requires
-      R.valid r)
+      R.valid p)
     (ensures fun h0 ht h1 ->
       B.modifies B.loc_none h0 h1 /\
-      ht == HSM.tag_of_handshake (R.value r))
-  = let open R in
-    let open Parsers.HandshakeType in
+      ht == HSM.tag_of_handshake (R.value p))
+  = let open Parsers.HandshakeType in
     R.reveal_valid();
-    let b = R.to_slice b in
-    handshakeType_reader b r.start_pos
+    let b = R.temp_slice_of_repr_ptr p in
+    handshakeType_reader b 0ul
 
-let is_ch (#b:R.const_slice) (r:repr b) : GTot bool =
-  HSM.M_client_hello? (R.value r)
+let is_ch (p:ptr) : GTot bool =
+  HSM.M_client_hello? (R.value p)
 
-let is_sh (#b:R.const_slice) (r:repr b) : GTot bool =
-  HSM.M_server_hello? (R.value r)
+let is_sh (p:ptr) : GTot bool =
+  HSM.M_server_hello? (R.value p)
 
-type ch_repr (b:R.const_slice) = m:repr b{is_ch m}
-type sh_repr (b:R.const_slice) = m:repr b{is_sh m}
+type ch_ptr = m:ptr{is_ch m}
+type sh_ptr = m:ptr{is_sh m}
 
-let clientHello (#b:R.const_slice) (r:repr b{is_ch r})
-  : Stack (RCH.repr b)
+let clientHello (r:ch_ptr)
+  : Stack RCH.ptr
     (requires fun h ->
       R.valid r h)
     (ensures fun h0 ch h1 ->
       B.modifies B.loc_none h0 h1 /\
       R.valid ch h1 /\
-      R.value ch == HSM.M_client_hello?._0 (R.value r))
+      R.value ch == HSM.M_client_hello?._0 (R.value r) /\
+      ch `R.sub_ptr` r)
   = let open R in
     let open Parsers.HandshakeType in
     R.reveal_valid();
     let h = get () in
-    let s = R.to_slice b in
-    let pos = HSM.handshake_accessor_client_hello s r.start_pos in
+    let s = R.temp_slice_of_repr_ptr r in
+    let pos = HSM.handshake_accessor_client_hello s 0ul in
     let pos = HSM.handshake_m_client_hello_accessor s pos in
     let end_pos = Parsers.ClientHello.clientHello_jumper s pos in
-    let ch_repr = R.mk_from_const_slice b pos end_pos Parsers.ClientHello.clientHello_parser32 in
-    ch_repr
+    let ch = R.mk s pos end_pos Parsers.ClientHello.clientHello_parser32 in
+    R.intro_sub_ptr ch r pos end_pos;
+    ch
 
-let serverHello (#b:R.const_slice) (r:repr b{is_sh r})
-  : Stack (RSH.repr b)
+let serverHello (r:sh_ptr)
+  : Stack RSH.ptr
     (requires fun h ->
       R.valid r h)
     (ensures fun h0 sh h1 ->
       B.modifies B.loc_none h0 h1 /\
       R.valid sh h1 /\
-      R.value sh == HSM.M_server_hello?._0 (R.value r))
+      R.value sh == HSM.M_server_hello?._0 (R.value r) /\
+      sh `R.sub_ptr` r)
   = let open R in
     let open Parsers.HandshakeType in
     R.reveal_valid();
     let h = get () in
-    let s = R.to_slice b in
-    let pos = HSM.handshake_accessor_server_hello s r.start_pos in
+    let s = R.temp_slice_of_repr_ptr r in
+    let pos = HSM.handshake_accessor_server_hello s 0ul in
     let pos = HSM.handshake_m_server_hello_accessor s pos in
     let end_pos = Parsers.ServerHello.serverHello_jumper s pos in
-    let sh_repr = R.mk_from_const_slice b pos end_pos Parsers.ServerHello.serverHello_parser32 in
-    sh_repr
+    let sh = R.mk s pos end_pos Parsers.ServerHello.serverHello_parser32 in
+    R.intro_sub_ptr sh r pos end_pos;
+    sh
 
 (* Serializer from high-level value via intermediate-level formatter *)
 
-let serialize
-  (b:LP.slice R.mut_p R.mut_p{ LP.(b.len <= validator_max_length) })
-  (from:R.index (R.of_slice b))
-  (x: t)
-: Stack (option (repr (R.of_slice b)))
+let serialize (b:LP.slice R.mut_p R.mut_p{ LP.(b.len <= validator_max_length) })
+              (from:R.index (R.of_slice b))
+              (x:t)
+  : Stack (option (pos (R.of_slice b)))
     (requires fun h ->
       LP.live_slice h b)
     (ensures fun h0 r h1 ->
       B.modifies (LP.loc_slice_from b from) h0 h1 /\
-      begin match r with
+      begin
+      match r with
       | None ->
         (* not enough space in output slice *)
         Seq.length (LP.serialize HSM.handshake_serializer x) > FStar.UInt32.v (b.LP.len - from)
       | Some r ->
-        R.valid r h1 /\
+        R.repr_pos_valid r h1 /\
         r.R.start_pos == from /\
-        R.value r == x
-      end
-    )
-= R.mk_from_serialize b from HSM.handshake_parser32 HSM.handshake_serializer32 HSM.handshake_size32 x
+        R.value_pos r == x
+      end)
+  = R.mk_repr_pos_from_serialize b from HSM.handshake_parser32 HSM.handshake_serializer32 HSM.handshake_size32 x
